isolation/Isolation.v
@@ -1,0 +1,369 @@
+From compcert Require Import Integers Values.
+From bpf.comm Require Import State Monad.
+From bpf.model Require Import Syntax Semantics.
+From bpf.isolation Require Import CommonLib AlignChunk RegsInv MemInv IsolationLemma.
+
+From Coq Require Import ZArith Lia.
+
+Open Scope Z_scope.
+
+Theorem step_preserving_inv:
+  forall st1 st2
+    (Hreg: register_inv st1)
+    (Hmem: memory_inv st1)
+    (Hsem: step st1 = Some (tt, st2)),
+       register_inv st2 /\ memory_inv st2.
+Proof.
+  unfold step.
+  unfold_monad.
+  intros.
+  destruct (Decode.decode _) in Hsem.
+  - (* BPF_NEG *)
+    apply reg_inv_eval_reg with (r:= r) in Hreg as Heval_reg.
+    destruct Heval_reg as (vl & Heval_reg).
+    destruct a; rewrite Heval_reg in Hsem; simpl in Hsem.
+    + split.
+      inversion Hsem.
+      eapply reg_inv_upd_reg; eauto.
+      eapply mem_inv_upd_reg; eauto.
+      inversion Hsem.
+      reflexivity.
+    + split.
+      inversion Hsem.
+      eapply reg_inv_upd_reg; eauto.
+      eapply mem_inv_upd_reg; eauto.
+      inversion Hsem.
+      reflexivity.
+  - (* BPF_BINARY *)
+    eapply step_preserving_inv_alu; eauto.
+  - (* BPF_JA *)
+    inversion Hsem; clear Hsem.
+    split; [eapply reg_inv_upd_pc; eauto | eapply mem_inv_upd_pc; eauto].
+  - (* BPF_JUMP *)
+    eapply step_preserving_inv_branch; eauto.
+  - (* BPF_LDDW *)
+    destruct Int.lt; simpl in Hsem.
+    unfold Int64.iwordsize', Int64.zwordsize, Int64.wordsize, Wordsize_64.wordsize in Hsem; simpl in Hsem.
+    unfold Int.ltu in Hsem.
+    rewrite Int.unsigned_repr in Hsem; [idtac| rewrite Int_max_unsigned_eq; lia].
+    rewrite Int.unsigned_repr in Hsem; [idtac| rewrite Int_max_unsigned_eq; lia].
+    simpl in Hsem.
+
+    inversion Hsem; clear Hsem.
+    + split.
+      apply reg_inv_upd_pc_incr with (st1:= (State.upd_reg r
+          (Vlong
+             (Int64.or (Int64.repr (Int.signed i))
+                (Int64.shl'
+                   (Int64.repr
+                      (Int.signed
+                         (Regs.get_immediate
+                            (State.eval_ins
+                               (Int.add (State.eval_pc st1) Int.one) st1))))
+                   (Int.repr 32)))) st1)); auto.
+      eapply reg_inv_upd_reg; eauto.
+      apply mem_inv_upd_pc_incr with (st1:= (State.upd_reg r
+          (Vlong
+             (Int64.or (Int64.repr (Int.signed i))
+                (Int64.shl'
+                   (Int64.repr
+                      (Int.signed
+                         (Regs.get_immediate
+                            (State.eval_ins
+                               (Int.add (State.eval_pc st1) Int.one) st1))))
+                   (Int.repr 32)))) st1)); auto.
+    + inversion Hsem; split; [eapply reg_inv_upd_flag; eauto | eapply mem_inv_upd_flag; eauto].
+  - (* BPF_LDX *)
+    eapply step_preserving_inv_ld; eauto.
+  - (* BPF_ST *)
+    eapply step_preserving_inv_st; eauto.
+  - (* BPF_RET *)
+    inversion Hsem.
+    split; [eapply reg_inv_upd_flag; eauto | eapply mem_inv_upd_flag; eauto].
+  - (* BPF_ERR *)
+    inversion Hsem.
+    split; [eapply reg_inv_upd_flag; eauto | eapply mem_inv_upd_flag; eauto].
+Qed.
+
+Theorem inv_avoid_undef:
+  forall st
+    (Hreg: register_inv st)
+    (Hmem: memory_inv st),
+      step st <> None.
+Proof.
+  intros.
+  unfold step.
+  unfold_monad.
+  destruct ( Decode.decode _).
+  - (* BPF_NEG *)
+    apply reg_inv_eval_reg with (r:= r) in Hreg as Heval_reg.
+    destruct Heval_reg as (vl & Heval_reg).
+    destruct a; rewrite Heval_reg; simpl; intro H ; inversion H.
+  - (* BPF_BINARY *)
+    unfold step_alu_binary_operation.
+    unfold_monad.
+    apply reg_inv_eval_reg with (r:= r) in Hreg as Heval_reg.
+    destruct Heval_reg as (vl & Heval_reg).
+    destruct a; rewrite Heval_reg; simpl; clear Heval_reg.
+    + destruct s.
+      apply reg_inv_eval_reg with (r:= r0) in Hreg as Heval_reg.
+      destruct Heval_reg as (vl0 & Heval_reg).
+      rewrite Heval_reg; simpl; clear Heval_reg.
+      destruct b; intro H; inversion H.
+      all: try (destruct negb eqn: Hnegb; [rewrite Bool.negb_true_iff in Hnegb; rewrite Hnegb in H1; simpl in H1; inversion H1 | rewrite Bool.negb_false_iff in Hnegb; inversion H1]).
+      all: try (clear H; destruct Int.ltu eqn: Hltu;
+       unfold Val.longofintu in H1; inversion H1).
+
+      destruct b; intro H; inversion H.
+      all: try (destruct negb eqn: Hnegb; [rewrite Bool.negb_true_iff in Hnegb; rewrite Hnegb in H1; simpl in H1; inversion H1 | rewrite Bool.negb_false_iff in Hnegb; inversion H1]).
+      all: try (clear H; destruct Int.ltu eqn: Hltu;
+       unfold Val.longofintu in H1; inversion H1).
+    + destruct s.
+      apply reg_inv_eval_reg with (r:= r0) in Hreg as Heval_reg.
+      destruct Heval_reg as (vl0 & Heval_reg).
+      rewrite Heval_reg; simpl; clear Heval_reg.
+      destruct b; intro H; inversion H.
+      all: try (destruct negb eqn: Hnegb; [rewrite Bool.negb_true_iff in Hnegb; rewrite Hnegb in H1; simpl in H1; inversion H1 | rewrite Bool.negb_false_iff in Hnegb; inversion H1]).
+      all: try (clear H; destruct Int.ltu eqn: Hltu;
+       unfold Val.longofintu in H1; inversion H1).
+
+      destruct b; intro H; inversion H.
+      all: try (destruct negb eqn: Hnegb; [rewrite Bool.negb_true_iff in Hnegb; rewrite Hnegb in H1; simpl in H1; inversion H1 | rewrite Bool.negb_false_iff in Hnegb; inversion H1]).
+      all: try (clear H; destruct Int.ltu eqn: Hltu;
+       unfold Val.longofintu in H1; inversion H1).
+  - (* BPF_JA *)
+    intro H; inversion H.
+  - (* BPF_JUMP *)
+    unfold step_branch_cond.
+    unfold_monad.
+    destruct s; destruct_if; intro H; inversion H.
+  - (* BPF_LDDW *)
+    destruct_if; intro H; inversion H.
+  - (* BPF_LDX *)
+    unfold step_load_x_operation.
+    unfold_monad.
+    unfold Val.addl.
+
+    apply reg_inv_eval_reg with (r:= r0) in Hreg as Heval_reg.
+    destruct Heval_reg as (vl & Heval_reg).
+    rewrite Heval_reg; clear Heval_reg.
+    unfold rBPFValues.sint32_to_vint.
+
+    assert (Hcheck_mem: exists ret, check_mem Memtype.Readable m
+    (rBPFValues.val_intuoflongu
+       match Val.longofint (Vint o) with
+       | Vlong n2 => Vlong (Int64.add vl n2)
+       | Vptr b2 ofs2 =>
+           if Archi.ptr64
+           then Vptr b2 (Ptrofs.add ofs2 (Ptrofs.of_int64 vl))
+           else Vundef
+       | _ => Vundef
+       end)
+    st = Some (ret, st)). {
+      eapply check_mem_same_state.
+    }
+    destruct Hcheck_mem as (ret & Hcheck_mem);
+    rewrite Hcheck_mem.
+    destruct rBPFValues.comp_eq_ptr8_zero eqn: Hptr; [intro H; inversion H|].
+
+    unfold load_mem, State.load_mem.
+    (**r from the fact Hptr and Hcheck_mem, we know Hwell_chunk *)
+    assert (Hwell_chunk: is_well_chunk m). {
+      unfold rBPFValues.comp_eq_ptr8_zero in Hptr.
+      unfold check_mem, bindM, returnM in Hcheck_mem.
+      Transparent Archi.ptr64.
+      destruct m; simpl in Hcheck_mem; inversion Hcheck_mem; unfold Vnullptr in *; subst; simpl in Hptr;
+      try (rewrite Int.eq_true in Hptr; inversion Hptr).
+      all: unfold is_well_chunk; constructor.
+    }
+    unfold State._to_vlong, Regs.val64_zero.
+    assert (Hneq: ret <> Vnullptr). {
+      unfold rBPFValues.comp_eq_ptr8_zero in Hptr.
+      unfold Vnullptr; simpl.
+      intro.
+      rewrite H in Hptr.
+      rewrite Int.eq_true in Hptr.
+      inversion Hptr.
+    }
+
+    unfold rBPFValues.val_intuoflongu, Val.longofint in Hcheck_mem.
+    destruct m.
+    all: try (intro H; inversion H).
+    all: eapply check_mem_load' in Hmem; eauto.
+    all: destruct Hmem as (res & Hmem & Hvlong_vint); clear H; rewrite Hmem in H1.
+    all: unfold is_vlong_or_vint in Hvlong_vint.
+    all: destruct res; try inversion Hvlong_vint; inversion H1.
+    unfold Memory.Mem.loadv in Hmem.
+    destruct ret; inversion Hmem.
+    eapply Memory.Mem.load_type in H0; eauto.
+  - (* BPF_ST *)
+    unfold step_store_operation.
+    unfold_monad.
+    unfold Val.addl.
+
+    destruct s.
+    +
+      apply reg_inv_eval_reg with (r:= r) in Hreg as Heval_reg.
+      destruct Heval_reg as (vl & Heval_reg).
+      rewrite Heval_reg; clear Heval_reg.
+
+      apply reg_inv_eval_reg with (r:= r0) in Hreg as Heval_reg.
+      destruct Heval_reg as (vl0 & Heval_reg).
+      rewrite Heval_reg; clear Heval_reg.
+      unfold rBPFValues.sint32_to_vint.
+
+      assert (Hcheck_mem: exists ret, check_mem Memtype.Writable m
+      (rBPFValues.val_intuoflongu
+       match Val.longofint (Vint o) with
+       | Vlong n2 => Vlong (Int64.add vl n2)
+       | Vptr b2 ofs2 =>
+           if Archi.ptr64
+           then Vptr b2 (Ptrofs.add ofs2 (Ptrofs.of_int64 vl))
+           else Vundef
+       | _ => Vundef
+       end)
+      st = Some (ret, st)). {
+        eapply check_mem_same_state.
+      }
+      destruct Hcheck_mem as (ret & Hcheck_mem);
+      rewrite Hcheck_mem.
+      destruct rBPFValues.comp_eq_ptr8_zero eqn: Hptr; [intro H; inversion H|].
+
+      unfold load_mem, State.load_mem.
+      (**r from the fact Hptr and Hcheck_mem, we know Hwell_chunk *)
+      assert (Hwell_chunk: is_well_chunk m). {
+        unfold rBPFValues.comp_eq_ptr8_zero in Hptr.
+        unfold check_mem, bindM, returnM in Hcheck_mem.
+        Transparent Archi.ptr64.
+        destruct m; simpl in Hcheck_mem; inversion Hcheck_mem; unfold Vnullptr in *; subst; simpl in Hptr;
+        try (rewrite Int.eq_true in Hptr; inversion Hptr).
+        all: unfold is_well_chunk; constructor.
+      }
+      unfold State._to_vlong, Regs.val64_zero.
+      assert (Hneq: ret <> Vnullptr). {
+        unfold rBPFValues.comp_eq_ptr8_zero in Hptr.
+        unfold Vnullptr; simpl.
+        intro.
+        rewrite H in Hptr.
+        rewrite Int.eq_true in Hptr.
+        inversion Hptr.
+      }
+
+      unfold rBPFValues.val_intuoflongu, Val.longofint in Hcheck_mem.
+      unfold store_mem_reg, State.store_mem_reg, State.vlong_to_vint_or_vlong.
+      assert (Heq: match m with
+    | AST.Mint8unsigned | AST.Mint16unsigned | AST.Mint32 | AST.Mint64 =>
+        match
+          Memory.Mem.storev m (bpf_m st) ret
+            match m with
+            | AST.Mint8unsigned | AST.Mint16unsigned | AST.Mint32 =>
+                Vint (Int.repr (Int64.unsigned vl0))
+            | AST.Mint64 => Vlong vl0
+            | _ => Vundef
+            end
+        with
+        | Some m0 => Some (upd_mem m0 st)
+        | None => None
+        end
+    | _ => Some (State.upd_flag Flag.BPF_ILLEGAL_MEM st)
+    end = match
+          Memory.Mem.storev m (bpf_m st) ret
+            match m with
+            | AST.Mint8unsigned | AST.Mint16unsigned | AST.Mint32 =>
+                Vint (Int.repr (Int64.unsigned vl0))
+            | AST.Mint64 => Vlong vl0
+            | _ => Vundef
+            end
+        with
+        | Some m0 => Some (upd_mem m0 st)
+        | None => None
+        end). {
+        destruct m; try inversion Hwell_chunk; try reflexivity.
+      }
+      rewrite Heq; clear Heq.
+      destruct m; try inversion Hwell_chunk.
+      all: eapply check_mem_store' with (v := Vlong vl0) in Hmem; eauto.
+      all: destruct Hmem as (m & Hstore & Hinv); unfold vlong_or_vint_to_vint_or_vlong, vlong_to_vint_or_vlong in Hstore; rewrite Hstore.
+      all: intro H; inversion H.
+    +
+      apply reg_inv_eval_reg with (r:= r) in Hreg as Heval_reg.
+      destruct Heval_reg as (vl & Heval_reg).
+      rewrite Heval_reg; clear Heval_reg.
+      unfold rBPFValues.sint32_to_vint.
+
+      assert (Hcheck_mem: exists ret, check_mem Memtype.Writable m
+      (rBPFValues.val_intuoflongu
+       match Val.longofint (Vint o) with
+       | Vlong n2 => Vlong (Int64.add vl n2)
+       | Vptr b2 ofs2 =>
+           if Archi.ptr64
+           then Vptr b2 (Ptrofs.add ofs2 (Ptrofs.of_int64 vl))
+           else Vundef
+       | _ => Vundef
+       end)
+      st = Some (ret, st)). {
+        eapply check_mem_same_state.
+      }
+      destruct Hcheck_mem as (ret & Hcheck_mem);
+      rewrite Hcheck_mem.
+      destruct rBPFValues.comp_eq_ptr8_zero eqn: Hptr; [intro H; inversion H|].
+
+      unfold load_mem, State.load_mem.
+      (**r from the fact Hptr and Hcheck_mem, we know Hwell_chunk *)
+      assert (Hwell_chunk: is_well_chunk m). {
+        unfold rBPFValues.comp_eq_ptr8_zero in Hptr.
+        unfold check_mem, bindM, returnM in Hcheck_mem.
+        Transparent Archi.ptr64.
+        destruct m; simpl in Hcheck_mem; inversion Hcheck_mem; unfold Vnullptr in *; subst; simpl in Hptr;
+        try (rewrite Int.eq_true in Hptr; inversion Hptr).
+        all: unfold is_well_chunk; constructor.
+      }
+      unfold State._to_vlong, Regs.val64_zero.
+      assert (Hneq: ret <> Vnullptr). {
+        unfold rBPFValues.comp_eq_ptr8_zero in Hptr.
+        unfold Vnullptr; simpl.
+        intro.
+        rewrite H in Hptr.
+        rewrite Int.eq_true in Hptr.
+        inversion Hptr.
+      }
+
+      unfold rBPFValues.val_intuoflongu, Val.longofint in Hcheck_mem.
+      unfold store_mem_imm, State.store_mem_imm, State.vint_to_vint_or_vlong.
+      assert (Heq: match m with
+    | AST.Mint8unsigned | AST.Mint16unsigned | AST.Mint32 | AST.Mint64 =>
+        match
+          Memory.Mem.storev m (bpf_m st) ret
+            match m with
+            | AST.Mint8unsigned | AST.Mint16unsigned | AST.Mint32 => Vint i
+            | AST.Mint64 => Vlong (Int64.repr (Int.unsigned i))
+            | _ => Vundef
+            end
+        with
+        | Some m0 => Some (upd_mem m0 st)
+        | None => None
+        end
+    | _ => Some (State.upd_flag Flag.BPF_ILLEGAL_MEM st)
+    end = match
+          Memory.Mem.storev m (bpf_m st) ret
+            match m with
+            | AST.Mint8unsigned | AST.Mint16unsigned | AST.Mint32 => Vint i
+            | AST.Mint64 => Vlong (Int64.repr (Int.unsigned i))
+            | _ => Vundef
+            end
+        with
+        | Some m0 => Some (upd_mem m0 st)
+        | None => None
+        end). {
+        destruct m; try inversion Hwell_chunk; try reflexivity.
+      }
+      rewrite Heq; clear Heq.
+      destruct m; try inversion Hwell_chunk.
+      all: eapply check_mem_store' with (v := Vint i) in Hmem; eauto.
+      all: destruct Hmem as (m & Hstore & Hinv); unfold vlong_or_vint_to_vint_or_vlong, vint_to_vint_or_vlong in Hstore; rewrite Hstore.
+      all: intro H; inversion H.
+  - (* BPF_RET *)
+    intro H; inversion H.
+  - (* BPF_ERR *)
+    intro H; inversion H.
+Qed.
