isolation/IsolationLemma.v
@@ -1,0 +1,1221 @@
+From compcert Require Import Integers Values Memory AST.
+From bpf.comm Require Import State Monad.
+From bpf.model Require Import Syntax Semantics.
+From bpf.isolation Require Import CommonLib AlignChunk RegsInv MemInv.
+
+From Coq Require Import ZArith List.
+Import ListNotations.
+
+Open Scope Z_scope.
+
+Ltac unfold_monad :=
+  match goal with
+  | |- _ =>
+    unfold eval_pc, eval_ins, eval_mrs_num, eval_mem, eval_mem_regions, get_addr_ofs, decodeM, upd_reg, upd_flag, eval_src32, eval_src, eval_reg32, upd_pc, upd_pc_incr, eval_reg, eval_ins_len, get_immediate, bindM, returnM
+  end.
+
+
+Ltac destruct_if :=
+  repeat match goal with
+  | |- context [if ?X then _ else _] =>
+    destruct X
+  end.
+
+Lemma step_preserving_inv_alu:
+  forall st1 st2 a b r s
+    (Hreg : register_inv st1)
+    (Hmem : memory_inv st1)
+    (Hsem : step_alu_binary_operation a b r s st1 = Some (tt, st2)),
+      register_inv st2 /\ memory_inv st2.
+Proof.
+  unfold step_alu_binary_operation; unfold_monad; intros.
+  apply reg_inv_eval_reg with (r := r) in Hreg as Heval_reg;
+  destruct Heval_reg as (src & Heval_reg).
+  destruct a; rewrite Heval_reg in Hsem; clear Heval_reg; simpl in Hsem.
+  - (**r A32 *)
+    destruct s.
+    + (**r inl r *)
+      apply reg_inv_eval_reg with (r := r0) in Hreg as Heval_reg;
+      destruct Heval_reg as (src0 & Heval_reg).
+      rewrite Heval_reg in Hsem; clear Heval_reg; simpl in Hsem.
+      destruct b; inversion Hsem; clear Hsem.
+      * split; [eapply reg_inv_upd_reg; eauto | eapply mem_inv_upd_reg; eauto].
+      * split; [eapply reg_inv_upd_reg; eauto | eapply mem_inv_upd_reg; eauto].
+      * split; [eapply reg_inv_upd_reg; eauto | eapply mem_inv_upd_reg; eauto].
+      * split; (destruct negb eqn: Hnegb; [rewrite Bool.negb_true_iff in Hnegb; rewrite Hnegb in H0; simpl in H0; inversion H0 | rewrite Bool.negb_false_iff in Hnegb; inversion H0]).
+        eapply reg_inv_upd_reg; eauto.
+        eapply reg_inv_upd_flag; eauto.
+        eapply mem_inv_upd_reg; eauto.
+        eapply mem_inv_upd_flag; eauto.
+      * split; [eapply reg_inv_upd_reg; eauto | eapply mem_inv_upd_reg; eauto].
+      * split; [eapply reg_inv_upd_reg; eauto | eapply mem_inv_upd_reg; eauto].
+      * split; destruct Int.ltu eqn: Hltu; simpl in H0; inversion H0; clear H0.
+        eapply reg_inv_upd_reg; eauto.
+        eapply reg_inv_upd_flag; eauto.
+        eapply mem_inv_upd_reg; eauto.
+        eapply mem_inv_upd_flag; eauto.
+      * split; destruct Int.ltu eqn: Hltu; simpl in H0; inversion H0; clear H0.
+        eapply reg_inv_upd_reg; eauto.
+        eapply reg_inv_upd_flag; eauto.
+        eapply mem_inv_upd_reg; eauto.
+        eapply mem_inv_upd_flag; eauto.
+      * split; (destruct negb eqn: Hnegb; [rewrite Bool.negb_true_iff in Hnegb; rewrite Hnegb in H0; simpl in H0; inversion H0 | rewrite Bool.negb_false_iff in Hnegb; inversion H0]).
+        eapply reg_inv_upd_reg; eauto.
+        eapply reg_inv_upd_flag; eauto.
+        eapply mem_inv_upd_reg; eauto.
+        eapply mem_inv_upd_flag; eauto.
+      * split; [eapply reg_inv_upd_reg; eauto | eapply mem_inv_upd_reg; eauto].
+      * split; [eapply reg_inv_upd_reg; eauto | eapply mem_inv_upd_reg; eauto].
+      * split; destruct Int.ltu eqn: Hltu; simpl in H0; inversion H0; clear H0.
+        eapply reg_inv_upd_reg; eauto.
+        eapply reg_inv_upd_flag; eauto.
+        eapply mem_inv_upd_reg; eauto.
+        eapply mem_inv_upd_flag; eauto.
+    + (**r inr i *)
+      destruct b; inversion Hsem; clear Hsem.
+      * split; [eapply reg_inv_upd_reg; eauto | eapply mem_inv_upd_reg; eauto].
+      * split; [eapply reg_inv_upd_reg; eauto | eapply mem_inv_upd_reg; eauto].
+      * split; [eapply reg_inv_upd_reg; eauto | eapply mem_inv_upd_reg; eauto].
+      * split; (destruct negb eqn: Hnegb; [rewrite Bool.negb_true_iff in Hnegb; rewrite Hnegb in H0; simpl in H0; inversion H0 | rewrite Bool.negb_false_iff in Hnegb; inversion H0]).
+        eapply reg_inv_upd_reg; eauto.
+        eapply reg_inv_upd_flag; eauto.
+        eapply mem_inv_upd_reg; eauto.
+        eapply mem_inv_upd_flag; eauto.
+      * split; [eapply reg_inv_upd_reg; eauto | eapply mem_inv_upd_reg; eauto].
+      * split; [eapply reg_inv_upd_reg; eauto | eapply mem_inv_upd_reg; eauto].
+      * split; destruct Int.ltu eqn: Hltu; simpl in H0; inversion H0; clear H0.
+        eapply reg_inv_upd_reg; eauto.
+        eapply reg_inv_upd_flag; eauto.
+        eapply mem_inv_upd_reg; eauto.
+        eapply mem_inv_upd_flag; eauto.
+      * split; destruct Int.ltu eqn: Hltu; simpl in H0; inversion H0; clear H0.
+        eapply reg_inv_upd_reg; eauto.
+        eapply reg_inv_upd_flag; eauto.
+        eapply mem_inv_upd_reg; eauto.
+        eapply mem_inv_upd_flag; eauto.
+      * split; (destruct negb eqn: Hnegb; [rewrite Bool.negb_true_iff in Hnegb; rewrite Hnegb in H0; simpl in H0; inversion H0 | rewrite Bool.negb_false_iff in Hnegb; inversion H0]).
+        eapply reg_inv_upd_reg; eauto.
+        eapply reg_inv_upd_flag; eauto.
+        eapply mem_inv_upd_reg; eauto.
+        eapply mem_inv_upd_flag; eauto.
+      * split; [eapply reg_inv_upd_reg; eauto | eapply mem_inv_upd_reg; eauto].
+      * split; [eapply reg_inv_upd_reg; eauto | eapply mem_inv_upd_reg; eauto].
+      * split; destruct Int.ltu eqn: Hltu; simpl in H0; inversion H0; clear H0.
+        eapply reg_inv_upd_reg; eauto.
+        eapply reg_inv_upd_flag; eauto.
+        eapply mem_inv_upd_reg; eauto.
+        eapply mem_inv_upd_flag; eauto.
+  - (**r A64 *)
+    destruct s.
+    + (**r inl r *)
+      apply reg_inv_eval_reg with (r := r0) in Hreg as Heval_reg;
+      destruct Heval_reg as (src0 & Heval_reg).
+      rewrite Heval_reg in Hsem; clear Heval_reg; simpl in Hsem.
+      destruct b; inversion Hsem; clear Hsem.
+      * split; [eapply reg_inv_upd_reg; eauto | eapply mem_inv_upd_reg; eauto].
+      * split; [eapply reg_inv_upd_reg; eauto | eapply mem_inv_upd_reg; eauto].
+      * split; [eapply reg_inv_upd_reg; eauto | eapply mem_inv_upd_reg; eauto].
+      * split; (destruct negb eqn: Hnegb; [rewrite Bool.negb_true_iff in Hnegb; rewrite Hnegb in H0; simpl in H0; inversion H0 | rewrite Bool.negb_false_iff in Hnegb; inversion H0]).
+        eapply reg_inv_upd_reg; eauto.
+        eapply reg_inv_upd_flag; eauto.
+        eapply mem_inv_upd_reg; eauto.
+        eapply mem_inv_upd_flag; eauto.
+      * split; [eapply reg_inv_upd_reg; eauto | eapply mem_inv_upd_reg; eauto].
+      * split; [eapply reg_inv_upd_reg; eauto | eapply mem_inv_upd_reg; eauto].
+      * split; destruct Int.ltu eqn: Hltu; simpl in H0; inversion H0; clear H0.
+        eapply reg_inv_upd_reg; eauto.
+        eapply reg_inv_upd_flag; eauto.
+        eapply mem_inv_upd_reg; eauto.
+        eapply mem_inv_upd_flag; eauto.
+      * split; destruct Int.ltu eqn: Hltu; simpl in H0; inversion H0; clear H0.
+        eapply reg_inv_upd_reg; eauto.
+        eapply reg_inv_upd_flag; eauto.
+        eapply mem_inv_upd_reg; eauto.
+        eapply mem_inv_upd_flag; eauto.
+      * split; (destruct negb eqn: Hnegb; [rewrite Bool.negb_true_iff in Hnegb; rewrite Hnegb in H0; simpl in H0; inversion H0 | rewrite Bool.negb_false_iff in Hnegb; inversion H0]).
+        eapply reg_inv_upd_reg; eauto.
+        eapply reg_inv_upd_flag; eauto.
+        eapply mem_inv_upd_reg; eauto.
+        eapply mem_inv_upd_flag; eauto.
+      * split; [eapply reg_inv_upd_reg; eauto | eapply mem_inv_upd_reg; eauto].
+      * split; [eapply reg_inv_upd_reg; eauto | eapply mem_inv_upd_reg; eauto].
+      * split; destruct Int.ltu eqn: Hltu; simpl in H0; inversion H0; clear H0.
+        eapply reg_inv_upd_reg; eauto.
+        eapply reg_inv_upd_flag; eauto.
+        eapply mem_inv_upd_reg; eauto.
+        eapply mem_inv_upd_flag; eauto.
+    + (**r inr i *)
+      destruct b; inversion Hsem; clear Hsem.
+      * split; [eapply reg_inv_upd_reg; eauto | eapply mem_inv_upd_reg; eauto].
+      * split; [eapply reg_inv_upd_reg; eauto | eapply mem_inv_upd_reg; eauto].
+      * split; [eapply reg_inv_upd_reg; eauto | eapply mem_inv_upd_reg; eauto].
+      * split; (destruct negb eqn: Hnegb; [rewrite Bool.negb_true_iff in Hnegb; rewrite Hnegb in H0; simpl in H0; inversion H0 | rewrite Bool.negb_false_iff in Hnegb; inversion H0]).
+        eapply reg_inv_upd_reg; eauto.
+        eapply reg_inv_upd_flag; eauto.
+        eapply mem_inv_upd_reg; eauto.
+        eapply mem_inv_upd_flag; eauto.
+      * split; [eapply reg_inv_upd_reg; eauto | eapply mem_inv_upd_reg; eauto].
+      * split; [eapply reg_inv_upd_reg; eauto | eapply mem_inv_upd_reg; eauto].
+      * split; destruct Int.ltu eqn: Hltu; simpl in H0; inversion H0; clear H0.
+        eapply reg_inv_upd_reg; eauto.
+        eapply reg_inv_upd_flag; eauto.
+        eapply mem_inv_upd_reg; eauto.
+        eapply mem_inv_upd_flag; eauto.
+      * split; destruct Int.ltu eqn: Hltu; simpl in H0; inversion H0; clear H0.
+        eapply reg_inv_upd_reg; eauto.
+        eapply reg_inv_upd_flag; eauto.
+        eapply mem_inv_upd_reg; eauto.
+        eapply mem_inv_upd_flag; eauto.
+      * split; (destruct negb eqn: Hnegb; [rewrite Bool.negb_true_iff in Hnegb; rewrite Hnegb in H0; simpl in H0; inversion H0 | rewrite Bool.negb_false_iff in Hnegb; inversion H0]).
+        eapply reg_inv_upd_reg; eauto.
+        eapply reg_inv_upd_flag; eauto.
+        eapply mem_inv_upd_reg; eauto.
+        eapply mem_inv_upd_flag; eauto.
+      * split; [eapply reg_inv_upd_reg; eauto | eapply mem_inv_upd_reg; eauto].
+      * split; [eapply reg_inv_upd_reg; eauto | eapply mem_inv_upd_reg; eauto].
+      * split; destruct Int.ltu eqn: Hltu; simpl in H0; inversion H0; clear H0.
+        eapply reg_inv_upd_reg; eauto.
+        eapply reg_inv_upd_flag; eauto.
+        eapply mem_inv_upd_reg; eauto.
+        eapply mem_inv_upd_flag; eauto.
+Qed.
+
+Lemma step_preserving_inv_branch:
+  forall st1 st2 c r s o
+    (Hreg : register_inv st1)
+    (Hmem : memory_inv st1)
+    (Hsem : match step_branch_cond c r s st1 with
+       | Some (x', st') =>
+           (if x'
+            then
+             fun st : state =>
+             Some
+               (tt, State.upd_pc (Integers.Int.add (State.eval_pc st1) o) st)
+            else fun st : state => Some (tt, st)) st'
+       | None => None
+       end = Some (tt, st2)),
+      register_inv st2 /\ memory_inv st2.
+Proof.
+  unfold step_branch_cond; unfold_monad; intros.
+  apply reg_inv_eval_reg with (r := r) in Hreg as Heval_reg;
+  destruct Heval_reg as (src & Heval_reg).
+  rewrite Heval_reg in Hsem; clear Heval_reg; simpl in Hsem.
+  destruct s.
+  - (**r inl r *)
+    apply reg_inv_eval_reg with (r := r0) in Hreg as Heval_reg;
+    destruct Heval_reg as (src0 & Heval_reg).
+    rewrite Heval_reg in Hsem; clear Heval_reg; simpl in Hsem.
+    destruct (match c with
+         | Eq => Int64.eq src src0
+         | Gt Ctypes.Signed => Int64.lt src0 src
+         | Gt Ctypes.Unsigned => Int64.ltu src0 src
+         | Ge Ctypes.Signed => negb (Int64.lt src src0)
+         | Ge Ctypes.Unsigned => negb (Int64.ltu src src0)
+         | Lt Ctypes.Signed => Int64.lt src src0
+         | Lt Ctypes.Unsigned => Int64.ltu src src0
+         | Le Ctypes.Signed => negb (Int64.lt src0 src)
+         | Le Ctypes.Unsigned => negb (Int64.ltu src0 src)
+         | SEt => negb (Int64.eq (Int64.and src src0) Int64.zero)
+         | Ne => negb (Int64.eq src src0)
+         end); inversion Hsem; clear Hsem.
+    + split; [eapply reg_inv_upd_pc; eauto | eapply mem_inv_upd_pc; eauto].
+    + subst; intuition.
+  - (**r inr i *)
+    destruct (match c with
+         | Eq => Int64.eq src (Int64.repr (Int.signed i))
+         | Gt Ctypes.Signed => Int64.lt (Int64.repr (Int.signed i)) src
+         | Gt Ctypes.Unsigned => Int64.ltu (Int64.repr (Int.signed i)) src
+         | Ge Ctypes.Signed => negb (Int64.lt src (Int64.repr (Int.signed i)))
+         | Ge Ctypes.Unsigned =>
+             negb (Int64.ltu src (Int64.repr (Int.signed i)))
+         | Lt Ctypes.Signed => Int64.lt src (Int64.repr (Int.signed i))
+         | Lt Ctypes.Unsigned => Int64.ltu src (Int64.repr (Int.signed i))
+         | Le Ctypes.Signed => negb (Int64.lt (Int64.repr (Int.signed i)) src)
+         | Le Ctypes.Unsigned =>
+             negb (Int64.ltu (Int64.repr (Int.signed i)) src)
+         | SEt =>
+             negb
+               (Int64.eq (Int64.and src (Int64.repr (Int.signed i)))
+                  Int64.zero)
+         | Ne => negb (Int64.eq src (Int64.repr (Int.signed i)))
+         end); inversion Hsem; clear Hsem.
+    + split; [eapply reg_inv_upd_pc; eauto | eapply mem_inv_upd_pc; eauto].
+    + subst; intuition.
+Qed.
+
+Lemma check_mem_same_state :
+  forall perm chunk addr st1,
+    exists ret,
+      check_mem perm chunk addr st1 = Some (ret, st1).
+Proof.
+  unfold check_mem, is_well_chunk_bool; unfold_monad; intros.
+  
+  assert (Hcheck_mem_aux: forall n p c v st mrs, exists v', check_mem_aux n p c v mrs st = Some (v', st)). {
+    intros.
+    induction n.
+    simpl.
+    unfold_monad.
+    eexists; reflexivity.
+    simpl.
+    unfold_monad.
+    destruct IHn as (v' & IHn).
+    unfold get_mem_region.
+    unfold_monad.
+    unfold eval_mrs_regions.
+    assert (Hcheck_mem_aux2: forall mr p c v st, exists v', check_mem_aux2 mr p c v st = Some (v', st)). {
+      intros.
+      unfold check_mem_aux2, is_well_chunk_bool, get_block_ptr, get_start_addr, get_block_size, get_sub, get_add, get_block_perm.
+      unfold_monad.
+      destruct v0; destruct_if.
+      all: eexists; try reflexivity.
+   }
+    specialize (Hcheck_mem_aux2 (MemRegion.MyMemRegionsIndexnat mrs n) p v c st).
+    destruct Hcheck_mem_aux2 as (v0 & Hcheck_mem_aux2).
+    rewrite Hcheck_mem_aux2; clear Hcheck_mem_aux2.
+    destruct rBPFValues.comp_eq_ptr8_zero.
+    + eexists; eauto.
+    + eexists; try reflexivity.
+  }
+  unfold eval_mrs_regions.
+  destruct chunk eqn:Hchunk; specialize (Hcheck_mem_aux (eval_mem_num st1) perm chunk addr st1 (State.eval_mem_regions st1));
+  destruct Hcheck_mem_aux as ( v0 & Hcheck_mem_aux).
+  all: try inversion Hcheck_mem; try (eexists; reflexivity).
+  all: subst; rewrite Hcheck_mem_aux.
+  all: destruct rBPFValues.comp_eq_ptr8_zero; eexists; reflexivity.
+Qed.
+
+Lemma step_preserving_inv_ld:
+  forall st1 st2 m r r0 o
+    (Hreg : register_inv st1)
+    (Hmem : memory_inv st1)
+    (Hsem : step_load_x_operation m r r0 o st1 = Some (tt, st2)),
+      register_inv st2 /\ memory_inv st2.
+Proof.
+  unfold step_load_x_operation; unfold_monad; intros.
+  apply reg_inv_eval_reg with (r := r0) in Hreg as Heval_reg;
+  destruct Heval_reg as (src & Heval_reg).
+  rewrite Heval_reg in Hsem; clear Heval_reg; simpl in Hsem.
+  assert (Hcheck_mem: exists ret, check_mem Memtype.Readable m
+           (Vint
+              (Int.repr
+                 (Int64.unsigned (Int64.add src (Int64.repr (Int.signed o))))))
+           st1 = Some (ret, st1)). {
+    eapply check_mem_same_state.
+  }
+  destruct Hcheck_mem as (ret & Hcheck_mem); rewrite Hcheck_mem in Hsem; clear Hcheck_mem.
+  destruct rBPFValues.comp_eq_ptr8_zero; inversion Hsem; clear Hsem.
+  split; [eapply reg_inv_upd_flag; eauto | eapply mem_inv_upd_flag; eauto].
+  destruct State.load_mem in H0; inversion H0.
+  split; [eapply reg_inv_upd_reg; eauto | eapply mem_inv_upd_reg; eauto].
+Qed.
+
+Lemma step_preserving_inv_st:
+  forall st1 st2 m r s o
+    (Hreg : register_inv st1)
+    (Hmem : memory_inv st1)
+    (Hsem : step_store_operation m r s o st1 = Some (tt, st2)),
+      register_inv st2 /\ memory_inv st2.
+Proof.
+  unfold step_store_operation; unfold_monad; intros.
+  assert (Hcheck_mem: exists ret, check_mem Memtype.Writable m
+         (rBPFValues.val_intuoflongu
+            (Val.addl (State.eval_reg r st1)
+               (Val.longofint (rBPFValues.sint32_to_vint o)))) st1 = Some (ret, st1)). {
+    eapply check_mem_same_state.
+  }
+
+
+  destruct s.
+  - (**r inl r *)
+    destruct Hcheck_mem as (ret & Hcheck_mem); rewrite Hcheck_mem in Hsem.
+    destruct rBPFValues.comp_eq_ptr8_zero eqn: Hptr.
+    + inversion Hsem; clear Hsem.
+      split; [eapply reg_inv_upd_flag; eauto | eapply mem_inv_upd_flag; eauto].
+    +
+      (**r from the fact Hptr and Hcheck_mem, we know Hwell_chunk *)
+      assert (Hwell_chunk: is_well_chunk m). {
+        unfold rBPFValues.comp_eq_ptr8_zero in Hptr.
+        unfold check_mem, bindM, returnM in Hcheck_mem.
+        Transparent Archi.ptr64.
+        destruct m; simpl in Hcheck_mem; inversion Hcheck_mem; unfold Vnullptr in *; subst; simpl in Hptr;
+        try (rewrite Int.eq_true in Hptr; inversion Hptr).
+        all: unfold is_well_chunk; constructor.
+      }
+      apply reg_inv_eval_reg with (r := r0) in Hreg as Heval_reg;
+      destruct Heval_reg as (src & Heval_reg).
+      rewrite Heval_reg in Hsem; clear Heval_reg; simpl in Hsem.
+      unfold store_mem_reg in Hsem.
+      destruct State.store_mem_reg eqn: Hstore; [| inversion Hsem].
+      inversion Hsem; subst.
+      split; [eapply reg_inv_store_reg; eauto | eapply mem_inv_store_reg; eauto].
+  - (**r inr i *)
+    destruct Hcheck_mem as (ret & Hcheck_mem); rewrite Hcheck_mem in Hsem.
+    destruct rBPFValues.comp_eq_ptr8_zero eqn: Hptr.
+    + inversion Hsem; clear Hsem.
+      split; [eapply reg_inv_upd_flag; eauto | eapply mem_inv_upd_flag; eauto].
+    +
+      (**r from the fact Hptr and Hcheck_mem, we know Hwell_chunk *)
+      assert (Hwell_chunk: is_well_chunk m). {
+        unfold rBPFValues.comp_eq_ptr8_zero in Hptr.
+        unfold check_mem, bindM, returnM in Hcheck_mem.
+        Transparent Archi.ptr64.
+        destruct m; simpl in Hcheck_mem; inversion Hcheck_mem; unfold Vnullptr in *; subst; simpl in Hptr;
+        try (rewrite Int.eq_true in Hptr; inversion Hptr).
+        all: unfold is_well_chunk; constructor.
+      }
+      unfold rBPFValues.sint32_to_vint, store_mem_imm in Hsem.
+      destruct State.store_mem_imm eqn: Hstore; [| inversion Hsem].
+      inversion Hsem; subst.
+      split; [eapply reg_inv_store_imm; eauto | eapply mem_inv_store_imm; eauto].
+Qed.
+
+Definition is_well_chunk_boolP (chunk: memory_chunk) : bool :=
+  match chunk with
+  | Mint8unsigned | Mint16unsigned | Mint32 | Mint64 => true
+  | _ => false
+  end.
+
+Lemma is_well_chunk_boolM_P:
+  forall chunk st,
+    is_well_chunk_bool chunk st = Some (is_well_chunk_boolP chunk, st).
+Proof.
+  unfold is_well_chunk_bool, is_well_chunk_boolP.
+  unfold_monad.
+  intros.
+  destruct chunk; reflexivity.
+Qed.
+
+From bpf.comm Require Import MemRegion rBPFMemType rBPFAST rBPFValues.
+
+Definition check_mem_aux2P (mr: memory_region) (perm: permission) (addr: val) (chunk: memory_chunk): val :=
+  if is_well_chunk_boolP chunk then
+    let ptr    := block_ptr mr in
+    let start  := start_addr mr in
+    let size   := block_size mr in
+    let lo_ofs := Val.sub addr start in
+    let hi_ofs := Val.add lo_ofs (memory_chunk_to_valu32 chunk) in
+      if (andb (compu_le_32 Vzero lo_ofs) (compu_lt_32 hi_ofs size)) then
+        if (andb (compu_le_32 lo_ofs (memory_chunk_to_valu32_upbound chunk))
+                 (comp_eq_32 Vzero (val32_modu lo_ofs (memory_chunk_to_valu32 chunk)))) then
+            let mr_perm  := block_perm mr in
+              if (perm_ge mr_perm perm) then
+                Val.add ptr lo_ofs
+              else
+                Vnullptr
+          else
+            Vnullptr (**r = 0 *)
+        else
+          Vnullptr
+    else
+      Vnullptr.
+
+(*
+Lemma check_mem_aux2P_ptr:
+  forall mr perm addr chunk st1
+    (Hmem_inv: memory_inv st1),
+    (exists b ofs, check_mem_aux2P mr perm addr chunk = Vptr b ofs) \/  check_mem_aux2P mr perm addr chunk = Vnullptr.
+Proof.
+  intros.
+  unfold check_mem_aux2P.
+  destruct_if; intuition.
+  unfold memory_inv, inv_memory_regions in Hmem_inv.
+  unfold 
+  left. eexists;
+Qed.*)
+
+Lemma check_mem_aux2M_P:
+  forall mr perm addr chunk st,
+    check_mem_aux2 mr perm addr chunk st = Some (check_mem_aux2P mr perm addr chunk, st).
+Proof.
+  unfold check_mem_aux2, check_mem_aux2P.
+  unfold get_block_ptr, get_start_addr, get_block_size, get_sub, get_add, get_block_perm.
+  unfold_monad.
+  intros.
+  rewrite is_well_chunk_boolM_P.
+  destruct_if; reflexivity.
+Qed.
+
+Fixpoint check_mem_auxP (num: nat) (perm: permission) (chunk: memory_chunk) (addr: val) (mrs: MyMemRegionsType) {struct num}: val :=
+  match num with
+  | O => Vnullptr
+  | S n =>
+    let cur_mr    := MyMemRegionsIndexnat mrs n in
+    let check_mem := check_mem_aux2P cur_mr perm addr chunk in
+      if comp_eq_ptr8_zero check_mem then
+        check_mem_auxP n perm chunk addr mrs
+      else
+        check_mem
+  end.
+
+Lemma check_mem_auxM_P:
+  forall n perm chunk addr st mrs,
+    check_mem_aux n perm chunk addr mrs st = Some (check_mem_auxP n perm chunk addr mrs, st).
+Proof.
+  unfold check_mem_aux, get_mem_region, eval_mrs_regions, check_mem_auxP.
+  unfold_monad.
+  intros.
+  induction n.
+  reflexivity.
+  rewrite check_mem_aux2M_P.
+  destruct_if; try reflexivity.
+  rewrite IHn.
+  reflexivity.
+Qed.
+
+Definition check_memP (perm: permission) (chunk: memory_chunk) (addr: val) (st: State.state): val :=
+  let well_chunk := is_well_chunk_boolP chunk in
+    if well_chunk then
+      let mem_reg_num := eval_mem_num st in
+      let mrs         := State.eval_mem_regions st in
+      let check_mem  := check_mem_auxP mem_reg_num perm chunk addr mrs in
+        if comp_eq_ptr8_zero check_mem then
+          Vnullptr
+        else
+          check_mem
+    else
+      Vnullptr.
+
+Lemma check_memM_P:
+  forall perm chunk addr st,
+    check_mem perm chunk addr st = Some (check_memP perm chunk addr st, st).
+Proof.
+  unfold check_mem, eval_mrs_num, eval_mrs_regions, check_memP.
+  unfold_monad.
+  intros.
+  rewrite is_well_chunk_boolM_P.
+  destruct is_well_chunk_boolP; try reflexivity.
+  rewrite check_mem_auxM_P.
+  destruct_if; try reflexivity.
+Qed.
+
+Lemma well_chunk_iff:
+  forall chunk,
+    is_well_chunk chunk <-> is_well_chunk_boolP chunk = true.
+Proof.
+  unfold is_well_chunk, is_well_chunk_boolP.
+  intros.
+  destruct chunk; split; try constructor; intro H; inversion H.
+Qed.
+
+Fixpoint check_mem_auxL (perm: permission) (chunk: memory_chunk) (addr: val) (mrs: list memory_region): val :=
+  match mrs with
+  | [] => Vnullptr
+  | hd :: tl =>
+    let check_mem := check_mem_aux2P hd perm addr chunk in
+      if comp_eq_ptr8_zero check_mem then
+        check_mem_auxL perm chunk addr tl
+      else
+        check_mem
+  end.
+
+Definition check_memL (perm: permission) (chunk: memory_chunk) (addr: val) (st: State.state): val :=
+  let well_chunk := is_well_chunk_boolP chunk in
+    if well_chunk then
+      let mem_reg_num := eval_mem_num st in
+      let mrs         := State.eval_mem_regions st in
+      let check_mem  := check_mem_auxP mem_reg_num perm chunk addr mrs in
+        if comp_eq_ptr8_zero check_mem then
+          Vnullptr
+        else
+          check_mem
+    else
+      Vnullptr.
+(*
+Lemma check_mem_auxP_L:
+  forall perm chunk addr l,
+    (*(Hlist: bpf_mrs st = List.rev l), *)
+    check_mem_auxP (List.length l) perm chunk addr l = check_mem_auxL perm chunk addr (List.rev l).
+Proof.
+  intros perm chunk addr l.
+  unfold check_mem_auxP.
+  unfold State.eval_mem_regions, MyMemRegionsIndexnat, Memory_regions.index_nat.
+  induction l.
+  intros.
+  simpl.
+
+  reflexivity.
+  simpl in *.
+
+  intros.
+  destruct (length l).
+  admit.
+
+  assert (Heq_a: (nth (length l) (bpf_mrs st) default_memory_region) = a). {
+    rewrite Hlist.
+    rewrite <- rev_length.
+    rewrite nth_middle with (l' := []).
+    reflexivity.
+  }
+  rewrite Heq_a; clear Heq_a.
+  destruct comp_eq_ptr8_zero; [| reflexivity].
+  rewrite Hlist.
+  simpl.
+  apply IHl.
+Qed.*)
+
+Lemma check_mem_aux2P_spec:
+  forall mr chunk st1 p base len b b0 vi ofs
+    (H0 : check_mem_aux2P mr p (Vint vi) chunk = Vptr b ofs)
+    (Hptr : block_ptr mr = Vptr b0 Ptrofs.zero)
+    (Hvalid : Mem.valid_block (bpf_m st1) b0)
+    (Hbyte : is_byte_block b0 (bpf_m st1))
+    (Hstar : start_addr mr = Vint base)
+    (Hsize : block_size mr = Vint len)
+    (Hperm : perm_order (block_perm mr) p)
+    (Hrange_perm : Mem.range_perm (bpf_m st1) b0 0 (Int.unsigned len) Cur (block_perm mr)),
+        is_well_chunk chunk /\
+        ofs = Ptrofs.of_int (Int.sub vi base) /\
+        b = b0 /\
+        0 <= (Ptrofs.unsigned ofs) + size_chunk chunk < Int.unsigned len /\
+        Mem.valid_access (bpf_m st1) chunk b (Ptrofs.unsigned ofs) (block_perm mr).
+Proof.
+  unfold check_mem_aux2P.
+  intros.
+  destruct is_well_chunk_boolP eqn: Hwell_chunk; [| inversion H0].
+  split.
+  apply well_chunk_iff.
+  assumption.
+
+  destruct ((compu_le_32 Vzero (Val.sub (Vint vi) (start_addr mr)) &&
+        compu_lt_32
+          (Val.add (Val.sub (Vint vi) (start_addr mr))
+             (memory_chunk_to_valu32 chunk)) (block_size mr))%bool) eqn: Hlow; [| inversion H0].
+  destruct ((compu_le_32 (Val.sub (Vint vi) (start_addr mr))
+          (memory_chunk_to_valu32_upbound chunk) &&
+        comp_eq_32 Vzero
+          (val32_modu (Val.sub (Vint vi) (start_addr mr))
+             (memory_chunk_to_valu32 chunk)))%bool) eqn: Hhigh; [| inversion H0].
+  destruct (perm_ge (block_perm mr) p); [| inversion H0].
+
+  Transparent Archi.ptr64.
+  rewrite Hptr, Hstar, Hsize in *.
+  unfold Val.add, Val.sub in H0.
+  simpl in H0.
+  rewrite Ptrofs.add_zero_l in H0.
+  inversion H0.
+  split.
+  reflexivity.
+
+  subst.
+  unfold compu_le_32, compu_lt_32, comp_eq_32, Vzero, Val.sub in *.
+  unfold memory_chunk_to_valu32, memory_chunk_to_valu32_upbound, Val.add in *.
+  rewrite Ptrofs.agree32_of_int; [| reflexivity].
+  (**r with the fact `is_well_chunk_boolP`, we get the following lemma *)
+  assert (Heq_well_chunk: well_chunk_Z chunk = size_chunk chunk). {
+    unfold is_well_chunk_boolP in Hwell_chunk.
+    destruct chunk; try inversion Hwell_chunk.
+    all: unfold well_chunk_Z, size_chunk; reflexivity.
+  }
+  rewrite Heq_well_chunk in *; clear Heq_well_chunk.
+  (**r b = b0 *)
+  split.
+  reflexivity.
+
+  (**r Hlow is for _ <= _ < _ and Hhigh is for valid_access *)
+  apply andb_prop in Hlow, Hhigh.
+  destruct Hlow as (Hlow1 & Hlow2).
+  destruct Hhigh as (Hhigh1 & Hhigh2).
+  apply (hi_ofs_max_unsigned (Int.sub vi base) chunk) in Hhigh1.
+  apply Clt_implies_Zlt_add in Hlow2 as Hlow2'; [| assumption].
+  split.
+  assumption.
+
+  apply Cle_implies_Zle in Hlow1.
+  apply Clt_implies_Zlt_add with (hi := len) in Hhigh1; [| assumption].
+  unfold Mem.valid_access.
+  split.
+  eapply range_perm_included; eauto.
+  apply Int_unsigned_ofs_size_chunk_ge_0.
+  intuition.
+
+  unfold val32_modu in Hhigh2.
+
+  rewrite <- well_chunk_iff in Hwell_chunk.
+  destruct Val.modu eqn: Hmod; [| inversion Hhigh2].
+  destruct v; try inversion Hhigh2.
+  unfold Val.modu in Hmod.
+  destruct Int.eq eqn: Hmod2; [inversion Hmod|].
+  eapply modu_zero_is_aligned; eauto.
+  inversion Hmod.
+  rewrite <- H2 in H1.
+  assumption.
+Qed.
+
+Lemma check_mem_aux2P_spec':
+  forall mr chunk st1 p base len b vi ptr
+    (H0 : check_mem_aux2P mr p (Vint vi) chunk = ptr)
+    (Hneq : ptr <> Vnullptr)
+    (Hptr : block_ptr mr = Vptr b Ptrofs.zero)
+    (Hvalid : Mem.valid_block (bpf_m st1) b)
+    (Hbyte : is_byte_block b (bpf_m st1))
+    (Hstar : start_addr mr = Vint base)
+    (Hsize : block_size mr = Vint len)
+    (Hperm : perm_order (block_perm mr) p)
+    (Hrange_perm : Mem.range_perm (bpf_m st1) b 0 (Int.unsigned len) Cur (block_perm mr)),
+      exists ofs,
+        is_well_chunk chunk /\
+        ofs = Ptrofs.of_int (Int.sub vi base) /\
+        0 <= (Ptrofs.unsigned ofs) + size_chunk chunk < Int.unsigned len /\
+        ptr = Vptr b ofs /\
+        Mem.valid_access (bpf_m st1) chunk b (Ptrofs.unsigned ofs) (block_perm mr).
+Proof.
+  unfold check_mem_aux2P.
+  intros.
+  destruct is_well_chunk_boolP eqn: Hwell_chunk; [| rewrite H0 in Hneq; exfalso; apply Hneq; reflexivity].
+  rewrite Hptr, Hstar, Hsize in *.
+  unfold Val.add, Val.sub in H0.
+  rewrite Ptrofs.add_zero_l in H0.
+  exists (Ptrofs.of_int (Int.sub vi base)).
+  split.
+  apply well_chunk_iff.
+  assumption.
+
+  destruct ((compu_le_32 Vzero (Vint (Int.sub vi base)) &&
+        compu_lt_32
+          match memory_chunk_to_valu32 chunk with
+          | Vint n2 => Vint (Int.add (Int.sub vi base) n2)
+          | Vptr b2 ofs2 =>
+              if Archi.ptr64
+              then Vundef
+              else Vptr b2 (Ptrofs.add ofs2 (Ptrofs.of_int (Int.sub vi base)))
+          | _ => Vundef
+          end (Vint len))%bool) eqn: Hlow; [| rewrite H0 in Hneq; exfalso; apply Hneq; reflexivity].
+  destruct ((compu_le_32 (Vint (Int.sub vi base))
+          (memory_chunk_to_valu32_upbound chunk) &&
+        comp_eq_32 Vzero
+          (val32_modu (Vint (Int.sub vi base)) (memory_chunk_to_valu32 chunk)))%bool) eqn: Hhigh; [| rewrite H0 in Hneq; exfalso; apply Hneq; reflexivity].
+  destruct (perm_ge (block_perm mr) p); [| rewrite H0 in Hneq; exfalso; apply Hneq; reflexivity].
+
+  Transparent Archi.ptr64.
+  simpl in H0.
+  inversion H0.
+  split.
+  reflexivity.
+
+  subst.
+  unfold compu_le_32, compu_lt_32, comp_eq_32, Vzero, Val.sub in *.
+  unfold memory_chunk_to_valu32, memory_chunk_to_valu32_upbound, Val.add in *.
+  rewrite Ptrofs.agree32_of_int; [| reflexivity].
+  (**r with the fact `is_well_chunk_boolP`, we get the following lemma *)
+  assert (Heq_well_chunk: well_chunk_Z chunk = size_chunk chunk). {
+    unfold is_well_chunk_boolP in Hwell_chunk.
+    destruct chunk; try inversion Hwell_chunk.
+    all: unfold well_chunk_Z, size_chunk; reflexivity.
+  }
+  rewrite Heq_well_chunk in *; clear Heq_well_chunk.
+
+  (**r Hlow is for _ <= _ < _ and Hhigh is for valid_access *)
+  apply andb_prop in Hlow, Hhigh.
+  destruct Hlow as (Hlow1 & Hlow2).
+  destruct Hhigh as (Hhigh1 & Hhigh2).
+  apply (hi_ofs_max_unsigned (Int.sub vi base) chunk) in Hhigh1.
+  apply Clt_implies_Zlt_add in Hlow2 as Hlow2'; [| assumption].
+  split.
+  assumption.
+
+  split.
+  reflexivity.
+
+  apply Cle_implies_Zle in Hlow1.
+  apply Clt_implies_Zlt_add with (hi := len) in Hhigh1; [| assumption].
+  unfold Mem.valid_access.
+  split.
+  eapply range_perm_included; eauto.
+  apply Int_unsigned_ofs_size_chunk_ge_0.
+  intuition.
+
+  unfold val32_modu in Hhigh2.
+
+  rewrite <- well_chunk_iff in Hwell_chunk.
+  destruct Val.modu eqn: Hmod; [| inversion Hhigh2].
+  destruct v; try inversion Hhigh2.
+  unfold Val.modu in Hmod.
+  destruct Int.eq eqn: Hmod2; [inversion Hmod|].
+  eapply modu_zero_is_aligned; eauto.
+  inversion Hmod.
+  rewrite <- H2 in H1.
+  assumption.
+Qed.
+
+Lemma check_mem_load:
+  forall chunk st1 vi b ofs
+    (Hwell_chunk : is_well_chunk chunk)
+    (Hmem_inv: memory_inv st1)
+    (Hcheck_mem: check_mem Readable chunk (Vint vi) st1 = Some ((Vptr b ofs), st1)),
+    exists res,
+      (Memory.Mem.loadv chunk (bpf_m st1) (Vptr b ofs) = Some res)/\
+      is_vlong_or_vint res.
+Proof.
+  intros.
+  rewrite check_memM_P in Hcheck_mem.
+  inversion Hcheck_mem; clear Hcheck_mem.
+
+  unfold check_memP in *.
+  rewrite well_chunk_iff in Hwell_chunk.
+  rewrite Hwell_chunk in *.
+  Transparent Archi.ptr64.
+  destruct comp_eq_ptr8_zero.
+  inversion H0.
+
+  unfold eval_mem_num, State.eval_mem_regions in *.
+
+  induction (mrs_num st1).
+  simpl in *.
+  inversion H0.
+
+  simpl in *.
+  destruct comp_eq_ptr8_zero.
+  apply IHn.
+  specialize (IHn H0).
+  assumption.
+  remember (MyMemRegionsIndexnat (bpf_mrs st1) n) as mr.
+
+  (**r we rely on the fact if Heqmr get the default memory region, check_mem_aux2P should return Vnullptr! *)
+  assert (Hdefault: check_mem_aux2P default_memory_region Readable (Vint vi) chunk = Vnullptr). {
+    unfold check_mem_aux2P, default_memory_region.
+    unfold start_addr, block_size, block_perm, block_ptr.
+    Transparent Archi.ptr64.
+    assert (Hnullptr: Vint Int.zero = Vnullptr). {
+      unfold Vnullptr; reflexivity.
+    }
+    rewrite <- Hnullptr; clear Hnullptr.
+    assert (Hperm: perm_ge Nonempty Readable = false). {
+      unfold perm_ge.
+      unfold Mem.perm_order_dec.
+      reflexivity.
+    }
+    rewrite Hperm; clear Hperm.
+    destruct_if; try reflexivity.
+  }
+  rewrite H0.
+
+  unfold memory_inv in Hmem_inv.
+  unfold MyMemRegionsIndexnat in Heqmr.
+
+  unfold State.eval_mem_regions, Memory_regions.index_nat in Heqmr.
+  assert (Hin_mem_regions: List.In mr (bpf_mrs st1)). {
+    destruct nth_error eqn: Hnth_error.
+    + apply List.nth_error_In in Hnth_error.
+      subst.
+      assumption.
+    + subst.
+      rewrite Hdefault in H0.
+      inversion H0.
+  }
+  (**r now we get the evidence `In mr (bpf_mrs st1)`, and reuse the lemma `In_inv_memory_regions` *)
+  apply In_inv_memory_regions with (m:=bpf_m st1) in Hin_mem_regions; [| intuition].
+  assert (Hin_mem_regions' := Hin_mem_regions).
+  unfold inv_memory_region in Hin_mem_regions'.
+
+  destruct Hin_mem_regions' as (b0 & Hptr & Hvalid & Hbyte & base & len & Hstar & Hsize & Hperm & Hrange_perm).
+  eapply check_mem_aux2P_spec in H0; eauto.
+  destruct H0 as (Hwell_chunk' & Hofs & Hb_eq & Hofs_range & Hvalid_access).
+  subst b0.
+
+  apply Mem.valid_access_implies with (p2:= Readable) in Hvalid_access; [| assumption].
+  apply Mem.valid_access_load in Hvalid_access.
+  destruct Hvalid_access as (v & Hload).
+  exists v.
+  split; [unfold Mem.loadv; assumption | ].
+
+  assert (Hofs_range_c: 0 <= Ptrofs.unsigned ofs /\ Ptrofs.unsigned ofs + size_chunk chunk < Int.unsigned len). {
+      split.
+      apply ptrofs_unsigned_ge_0.
+      destruct Hofs_range as [Ha Hb]; assumption.
+    }
+
+  eapply load_some_well_chunk_vlong_or_vint; eauto.
+Qed.
+
+Lemma check_mem_load':
+  forall chunk st1 vi pt
+    (Hwell_chunk : is_well_chunk chunk)
+    (Hmem_inv: memory_inv st1)
+    (Hcheck_mem: check_mem Readable chunk (Vint vi) st1 = Some (pt, st1))
+    (Hneq: pt <> Vnullptr),
+    exists res,
+      (Memory.Mem.loadv chunk (bpf_m st1) pt = Some res)/\
+      is_vlong_or_vint res.
+Proof.
+  intros.
+  rewrite check_memM_P in Hcheck_mem.
+  inversion Hcheck_mem; clear Hcheck_mem.
+
+  unfold check_memP in *.
+  rewrite well_chunk_iff in Hwell_chunk.
+  rewrite Hwell_chunk in *.
+  Transparent Archi.ptr64.
+  destruct comp_eq_ptr8_zero.
+  rewrite H0 in Hneq.
+  exfalso; apply Hneq; reflexivity.
+
+  unfold eval_mem_num, State.eval_mem_regions in *.
+
+  induction (mrs_num st1).
+  simpl in *.
+  rewrite H0 in Hneq.
+  exfalso; apply Hneq; reflexivity.
+
+  simpl in *.
+  
+  destruct comp_eq_ptr8_zero.
+  apply IHn.
+  specialize (IHn H0).
+  assumption.
+  remember (MyMemRegionsIndexnat (bpf_mrs st1) n) as mr.
+
+  (**r we rely on the fact if Heqmr get the default memory region, check_mem_aux2P should return Vnullptr! *)
+  assert (Hdefault: check_mem_aux2P default_memory_region Readable (Vint vi) chunk = Vnullptr). {
+    unfold check_mem_aux2P, default_memory_region.
+    unfold start_addr, block_size, block_perm, block_ptr.
+    Transparent Archi.ptr64.
+    assert (Hnullptr: Vint Int.zero = Vnullptr). {
+      unfold Vnullptr; reflexivity.
+    }
+    rewrite <- Hnullptr; clear Hnullptr.
+    assert (Hperm: perm_ge Nonempty Readable = false). {
+      unfold perm_ge.
+      unfold Mem.perm_order_dec.
+      reflexivity.
+    }
+    rewrite Hperm; clear Hperm.
+    destruct_if; try reflexivity.
+  }
+  rewrite H0.
+
+  unfold memory_inv in Hmem_inv.
+  unfold MyMemRegionsIndexnat in Heqmr.
+
+  unfold State.eval_mem_regions, Memory_regions.index_nat in Heqmr.
+  assert (Hin_mem_regions: List.In mr (bpf_mrs st1)). {
+    destruct nth_error eqn: Hnth_error.
+    + apply List.nth_error_In in Hnth_error.
+      subst.
+      assumption.
+    + subst.
+      rewrite Hdefault in Hneq.
+      exfalso; apply Hneq; reflexivity.
+  }
+  (**r now we get the evidence `In mr (bpf_mrs st1)`, and reuse the lemma `In_inv_memory_regions` *)
+  apply In_inv_memory_regions with (m:=bpf_m st1) in Hin_mem_regions; [| intuition].
+  assert (Hin_mem_regions' := Hin_mem_regions).
+  unfold inv_memory_region in Hin_mem_regions'.
+
+  destruct Hin_mem_regions' as (b0 & Hptr & Hvalid & Hbyte & base & len & Hstar & Hsize & Hperm & Hrange_perm).
+  eapply check_mem_aux2P_spec' in H0; eauto.
+  destruct H0 as (ofs & Hwell_chunk' & Hofs & Hofs_range & Hptr_eq & Hvalid_access).
+
+  subst pt.
+  apply Mem.valid_access_implies with (p2:= Readable) in Hvalid_access; [| assumption].
+  apply Mem.valid_access_load in Hvalid_access.
+  destruct Hvalid_access as (v & Hload).
+  exists v.
+  unfold Mem.loadv.
+  split; [assumption | ].
+
+  assert (Hofs_range_c: 0 <= Ptrofs.unsigned ofs /\ Ptrofs.unsigned ofs + size_chunk chunk < Int.unsigned len). {
+      split.
+      apply ptrofs_unsigned_ge_0.
+      destruct Hofs_range as [Ha Hb]; assumption.
+    }
+
+  eapply load_some_well_chunk_vlong_or_vint; eauto.
+Qed.
+
+Definition vlong_or_vint_to_vint_or_vlong (chunk: memory_chunk) (v: val): val :=
+  match v with
+  | Vlong n => vlong_to_vint_or_vlong chunk v
+  | Vint  n => vint_to_vint_or_vlong chunk v
+  | _       => Vundef
+  end.
+
+Lemma check_mem_store:
+  forall chunk st1 vi b ofs v
+    (Hwell_chunk : is_well_chunk chunk)
+    (Hmem_inv: memory_inv st1)
+    (Hvlong_vint: is_vlong_or_vint v)
+    (Hcheck_mem: check_mem Writable chunk (Vint vi) st1 = Some ((Vptr b ofs), st1)),
+    exists m,
+      (Mem.storev chunk (bpf_m st1) (Vptr b ofs) (vlong_or_vint_to_vint_or_vlong chunk v) = Some m)/\
+      memory_inv (upd_mem m st1).
+Proof.
+  intros.
+  rewrite check_memM_P in Hcheck_mem.
+  inversion Hcheck_mem; clear Hcheck_mem.
+
+  unfold check_memP in *.
+  rewrite well_chunk_iff in Hwell_chunk.
+  rewrite Hwell_chunk in *.
+  Transparent Archi.ptr64.
+  destruct comp_eq_ptr8_zero.
+  inversion H0.
+
+  unfold eval_mem_num, State.eval_mem_regions in *.
+
+  induction (mrs_num st1).
+  simpl in *.
+  inversion H0.
+
+  simpl in *.
+  destruct comp_eq_ptr8_zero.
+  apply IHn.
+  specialize (IHn H0).
+  assumption.
+  remember (MyMemRegionsIndexnat (bpf_mrs st1) n) as mr.
+
+  (**r we rely on the fact if Heqmr get the default memory region, check_mem_aux2P should return Vnullptr! *)
+  assert (Hdefault: check_mem_aux2P default_memory_region Writable (Vint vi) chunk = Vnullptr). {
+    unfold check_mem_aux2P, default_memory_region.
+    unfold start_addr, block_size, block_perm, block_ptr.
+    Transparent Archi.ptr64.
+    assert (Hnullptr: Vint Int.zero = Vnullptr). {
+      unfold Vnullptr; reflexivity.
+    }
+    rewrite <- Hnullptr; clear Hnullptr.
+    assert (Hperm: perm_ge Nonempty Writable = false). {
+      unfold perm_ge.
+      unfold Mem.perm_order_dec.
+      reflexivity.
+    }
+    rewrite Hperm; clear Hperm.
+    destruct_if; try reflexivity.
+  }
+  rewrite H0.
+
+  unfold memory_inv in Hmem_inv.
+  unfold MyMemRegionsIndexnat in Heqmr.
+
+  unfold State.eval_mem_regions, Memory_regions.index_nat in Heqmr.
+  assert (Hin_mem_regions: List.In mr (bpf_mrs st1)). {
+    destruct nth_error eqn: Hnth_error.
+    + apply List.nth_error_In in Hnth_error.
+      subst.
+      assumption.
+    + subst.
+      rewrite Hdefault in H0.
+      inversion H0.
+  }
+  (**r now we get the evidence `In mr (bpf_mrs st1)`, and reuse the lemma `In_inv_memory_regions` *)
+  apply In_inv_memory_regions with (m:=bpf_m st1) in Hin_mem_regions; [| intuition].
+  assert (Hperm_w: perm_order (block_perm mr) Writable). {
+    unfold check_mem_aux2P in H0.
+    rewrite Hwell_chunk in H0.
+    destruct ((compu_le_32 Vzero (Val.sub (Vint vi) (start_addr mr)) &&
+         compu_lt_32
+           (Val.add (Val.sub (Vint vi) (start_addr mr))
+              (memory_chunk_to_valu32 chunk)) (block_size mr))%bool); [| inversion H0].
+    destruct ((compu_le_32 (Val.sub (Vint vi) (start_addr mr))
+          (memory_chunk_to_valu32_upbound chunk) &&
+        comp_eq_32 Vzero
+          (val32_modu (Val.sub (Vint vi) (start_addr mr))
+             (memory_chunk_to_valu32 chunk)))%bool); [| inversion H0].
+    unfold perm_ge in H0.
+    destruct Mem.perm_order_dec eqn: Hp.
+    assumption.
+    inversion H0.
+  }
+
+  assert (Hin_mem_regions' := Hin_mem_regions).
+  unfold inv_memory_region in Hin_mem_regions'.
+
+  destruct Hin_mem_regions' as (b0 & Hptr & Hvalid & Hbyte & base & len & Hstar & Hsize & Hperm & Hrange_perm).
+  eapply check_mem_aux2P_spec in H0; eauto.
+  destruct H0 as (Hwell_chunk' & Hofs & Hb_eq & Hofs_range & Hvalid_access).
+  subst b0.
+
+  apply Mem.valid_access_implies with (p2:= Writable) in Hvalid_access; [| assumption].
+  eapply Mem.valid_access_store in Hvalid_access; eauto.
+  destruct Hvalid_access as (m2 & Hstore).
+  exists m2.
+  split; [ apply Hstore | ].
+
+  (**r prove the memory_inv *)
+  unfold is_vlong_or_vint in Hvlong_vint.
+  destruct v; inversion Hvlong_vint.
+
+  - apply mem_inv_store_imm with (st1 := st1) (st2:= upd_mem m2 st1) (addr:= Vptr b ofs) (i:= i) in Hwell_chunk'; auto.
+  unfold State.store_mem_imm, vint_to_vint_or_vlong.
+  assert (Heq: match chunk with
+| Mint8unsigned | Mint16unsigned | Mint32 | Mint64 =>
+    match
+      Mem.storev chunk (bpf_m st1) (Vptr b ofs)
+        match chunk with
+        | Mint8unsigned | Mint16unsigned | Mint32 => Vint i
+        | Mint64 => Vlong (Int64.repr (Int.unsigned i))
+        | _ => Vundef
+        end
+    with
+    | Some m => Some (upd_mem m st1)
+    | None => None
+    end
+| _ => Some (State.upd_flag Flag.BPF_ILLEGAL_MEM st1)
+end = match
+      Mem.storev chunk (bpf_m st1) (Vptr b ofs)
+        match chunk with
+        | Mint8unsigned | Mint16unsigned | Mint32 => Vint i
+        | Mint64 => Vlong (Int64.repr (Int.unsigned i))
+        | _ => Vundef
+        end
+    with
+    | Some m => Some (upd_mem m st1)
+    | None => None
+    end). {
+      destruct chunk; try inversion Hwell_chunk'; try reflexivity.
+    }
+    rewrite Heq; clear Heq.
+    unfold Mem.storev.
+    unfold vlong_or_vint_to_vint_or_vlong, vint_to_vint_or_vlong in Hstore.
+    rewrite Hstore.
+    reflexivity.
+  - unfold vlong_or_vint_to_vint_or_vlong, vlong_to_vint_or_vlong in Hstore.
+    apply mem_inv_store_reg with (st1 := st1) (st2:= upd_mem m2 st1) (addr:= Vptr b ofs) (src:= i) in Hwell_chunk'; auto.
+  unfold State.store_mem_reg, vlong_to_vint_or_vlong.
+    destruct chunk; try inversion Hwell_chunk'; simpl.
+    all: try (rewrite Hstore; reflexivity).
+Qed.
+
+Lemma check_mem_store':
+  forall chunk st1 vi v pt
+    (Hwell_chunk : is_well_chunk chunk)
+    (Hmem_inv: memory_inv st1)
+    (Hvlong_vint: is_vlong_or_vint v)
+    (Hcheck_mem: check_mem Writable chunk (Vint vi) st1 = Some (pt, st1))
+    (Hneq: pt <> Vnullptr),
+    exists m,
+      (Mem.storev chunk (bpf_m st1) pt (vlong_or_vint_to_vint_or_vlong chunk v) = Some m)/\
+      memory_inv (upd_mem m st1).
+Proof.
+  intros.
+  rewrite check_memM_P in Hcheck_mem.
+  inversion Hcheck_mem; clear Hcheck_mem.
+
+  unfold check_memP in *.
+  rewrite well_chunk_iff in Hwell_chunk.
+  rewrite Hwell_chunk in *.
+  Transparent Archi.ptr64.
+  destruct comp_eq_ptr8_zero.
+  rewrite H0 in Hneq; exfalso; apply Hneq; reflexivity.
+
+  unfold eval_mem_num, State.eval_mem_regions in *.
+
+  induction (mrs_num st1).
+  simpl in *.
+  rewrite H0 in Hneq; exfalso; apply Hneq; reflexivity.
+
+  simpl in *.
+  destruct comp_eq_ptr8_zero.
+  apply IHn.
+  specialize (IHn H0).
+  assumption.
+
+  remember (MyMemRegionsIndexnat (bpf_mrs st1) n) as mr.
+
+  (**r we rely on the fact if Heqmr get the default memory region, check_mem_aux2P should return Vnullptr! *)
+  assert (Hdefault: check_mem_aux2P default_memory_region Writable (Vint vi) chunk = Vnullptr). {
+    unfold check_mem_aux2P, default_memory_region.
+    unfold start_addr, block_size, block_perm, block_ptr.
+    Transparent Archi.ptr64.
+    assert (Hnullptr: Vint Int.zero = Vnullptr). {
+      unfold Vnullptr; reflexivity.
+    }
+    rewrite <- Hnullptr; clear Hnullptr.
+    assert (Hperm: perm_ge Nonempty Writable = false). {
+      unfold perm_ge.
+      unfold Mem.perm_order_dec.
+      reflexivity.
+    }
+    rewrite Hperm; clear Hperm.
+    destruct_if; try reflexivity.
+  }
+  rewrite H0.
+
+  unfold memory_inv in Hmem_inv.
+  unfold MyMemRegionsIndexnat in Heqmr.
+
+  unfold State.eval_mem_regions, Memory_regions.index_nat in Heqmr.
+  assert (Hin_mem_regions: List.In mr (bpf_mrs st1)). {
+    destruct nth_error eqn: Hnth_error.
+    + apply List.nth_error_In in Hnth_error.
+      subst.
+      assumption.
+    + subst.
+      rewrite Hdefault in Hneq; exfalso; apply Hneq; reflexivity.
+  }
+  (**r now we get the evidence `In mr (bpf_mrs st1)`, and reuse the lemma `In_inv_memory_regions` *)
+  apply In_inv_memory_regions with (m:=bpf_m st1) in Hin_mem_regions; [| intuition].
+  assert (Hperm_w: perm_order (block_perm mr) Writable). {
+    unfold check_mem_aux2P in H0.
+    rewrite Hwell_chunk in H0.
+    destruct ((compu_le_32 Vzero (Val.sub (Vint vi) (start_addr mr)) &&
+         compu_lt_32
+           (Val.add (Val.sub (Vint vi) (start_addr mr))
+              (memory_chunk_to_valu32 chunk)) (block_size mr))%bool); [| rewrite H0 in Hneq; exfalso; apply Hneq; reflexivity].
+    destruct ((compu_le_32 (Val.sub (Vint vi) (start_addr mr))
+          (memory_chunk_to_valu32_upbound chunk) &&
+        comp_eq_32 Vzero
+          (val32_modu (Val.sub (Vint vi) (start_addr mr))
+             (memory_chunk_to_valu32 chunk)))%bool); [| rewrite H0 in Hneq; exfalso; apply Hneq; reflexivity].
+    unfold perm_ge in H0.
+    destruct Mem.perm_order_dec eqn: Hp.
+    assumption.
+    rewrite H0 in Hneq; exfalso; apply Hneq; reflexivity.
+  }
+
+  assert (Hin_mem_regions' := Hin_mem_regions).
+  unfold inv_memory_region in Hin_mem_regions'.
+
+  destruct Hin_mem_regions' as (b0 & Hptr & Hvalid & Hbyte & base & len & Hstar & Hsize & Hperm & Hrange_perm).
+  eapply check_mem_aux2P_spec' in H0; eauto.
+  destruct H0 as (ofs & Hwell_chunk' & Hofs & Hofs_range & Hptr_eq & Hvalid_access).
+  subst pt.
+
+  apply Mem.valid_access_implies with (p2:= Writable) in Hvalid_access; [| assumption].
+  eapply Mem.valid_access_store in Hvalid_access; eauto.
+  destruct Hvalid_access as (m2 & Hstore).
+  exists m2.
+  split; [ apply Hstore | ].
+
+  (**r prove the memory_inv *)
+  unfold is_vlong_or_vint in Hvlong_vint.
+  destruct v; inversion Hvlong_vint.
+
+  - apply mem_inv_store_imm with (st1 := st1) (st2:= upd_mem m2 st1) (addr:= Vptr b0 ofs) (i:= i) in Hwell_chunk'; auto.
+  unfold State.store_mem_imm, vint_to_vint_or_vlong.
+  assert (Heq: match chunk with
+| Mint8unsigned | Mint16unsigned | Mint32 | Mint64 =>
+    match
+      Mem.storev chunk (bpf_m st1) (Vptr b0 ofs)
+        match chunk with
+        | Mint8unsigned | Mint16unsigned | Mint32 => Vint i
+        | Mint64 => Vlong (Int64.repr (Int.unsigned i))
+        | _ => Vundef
+        end
+    with
+    | Some m => Some (upd_mem m st1)
+    | None => None
+    end
+| _ => Some (State.upd_flag Flag.BPF_ILLEGAL_MEM st1)
+end = match
+      Mem.storev chunk (bpf_m st1) (Vptr b0 ofs)
+        match chunk with
+        | Mint8unsigned | Mint16unsigned | Mint32 => Vint i
+        | Mint64 => Vlong (Int64.repr (Int.unsigned i))
+        | _ => Vundef
+        end
+    with
+    | Some m => Some (upd_mem m st1)
+    | None => None
+    end). {
+      destruct chunk; try inversion Hwell_chunk'; try reflexivity.
+    }
+    rewrite Heq; clear Heq.
+    unfold Mem.storev.
+    unfold vlong_or_vint_to_vint_or_vlong, vint_to_vint_or_vlong in Hstore.
+    rewrite Hstore.
+    reflexivity.
+  - unfold vlong_or_vint_to_vint_or_vlong, vlong_to_vint_or_vlong in Hstore.
+    apply mem_inv_store_reg with (st1 := st1) (st2:= upd_mem m2 st1) (addr:= Vptr b0 ofs) (src:= i) in Hwell_chunk'; auto.
+  unfold State.store_mem_reg, vlong_to_vint_or_vlong.
+    destruct chunk; try inversion Hwell_chunk'; simpl.
+    all: try (rewrite Hstore; reflexivity).
+Qed.
