isolation/README.md
@@ -1,0 +1,67 @@
+# Isolation proof (Certirbpf ensures the sandboxing property)
+
+This folder is used to prove the isolation property of the proof model (rbpf-coq interpreter).
+
+*using the make command: `make isolation`*
+
+There are two target thoerems:
+
+```Coq
+(**r Isolation.v *)
+Theorem step_preserving_inv:
+  forall st1 st2
+    (Hreg: register_inv st1)
+    (Hmem: memory_inv st1)
+    (Hsem: step st1 = Some (tt, st2)),
+       register_inv st2 /\ memory_inv st2.
+       
+Theorem inv_avoid_undef:
+  forall st
+    (Hreg: register_inv st)
+    (Hmem: memory_inv st),
+      step st <> None.       
+```
+where `register_inv` is the register invariant and `memory_inv` is the memory invariant for Certirbpf.
+
+## File struct
+- `CommonLib.v`: some common lemmas
+- `AlignChunk.v`: some definitions and lemmas about **Memory Aligned**
+- `RegsInv.v`: the register invariant and related lemmas
+- `MemInv.v`: the memory invariant and related lemmas
+- `IsolationLemma.v`: some lemmas used by the proof of the isolation property
+- `Isolation.v`: two target thoerems.
+
+## Proof idea
+
+The whole way to prove the theorems are do case discussion on each instruction.
+
+But there is a gap between proof idea and code generation idea: To simulate `Coq List type` correctly, we define `comm/MemType.v/MyMemRegionsType` in Coq, it use List.nth_error to access a list. This way makes the code generation easier but complex the isolation proof. Because we have a list of memory regions `Coq List type`, when we define its invariants, it natually uses native Coq List constructions `nil` and `hd::tl`, but remember we are using `nth\_error` to access the list. So it is hard to do `induction` on the list.
+
+To solve this question, we use the relation among `List.In`, `List.nth_error` and Coq List constructions!
+- `inv_memory_regions` is defined by using Coq List constructions
+- `In_inv_memory_regions` says the relation between the former and `List.In`
+- `IsolationLemma.v` uses the relation with `List.nth_error`, and complete the proof.
+```Coq
+(**r MemInv.v *)
+Fixpoint inv_memory_regions (m:mem) (mrs: list memory_region): Prop :=
+  match mrs with
+  | [] => True
+  | hd :: tl => inv_memory_region m hd /\ inv_memory_regions m tl
+  end.
+
+Lemma In_inv_memory_regions:
+  forall mr m l,
+    List.In mr l -> inv_memory_regions m l ->
+      inv_memory_region m mr.
+Proof.
+
+(**r IsolationLemma.v L773 & L805 *)
+
+  (**r we rely on the fact if Heqmr get the default memory region, check_mem_aux2P should return Vnullptr! *)
+  assert (Hdefault: check_mem_aux2P default_memory_region Readable (Vint vi) chunk = Vnullptr). {
+  ...
+  
+  (**r now we get the evidence `In mr (bpf_mrs st1)`, and reuse the lemma `In_inv_memory_regions` *)
+  apply In_inv_memory_regions with (m:=bpf_m st1) in Hin_mem_regions; [| intuition].
+
+```
